tests/lean/run/coinductive.lean
@@ -3,8 +3,6 @@ import data.stream
 
 universe u
 
-open level expr tactic
-
 coinductive all_stream {α : Type u} (s : set α) : stream α → Prop
 | step {} : ∀{a : α} {ω : stream α}, a ∈ s → all_stream ω → all_stream (a :: ω)
 
@@ -17,6 +15,8 @@ coinductive all_stream {α : Type u} (s : set α) : stream α → Prop
   ∀ {α : Type u} (s : set α) (C : stream α → Prop),
     (∀ (a : stream α), C a → all_stream.functional s C a) → ∀ (a : stream α), C a → all_stream s a)
 
+coinductive all_stream' {α : Type u} (s : set α) : stream α → Prop
+| step {} : ∀{ω : stream α}, stream.head ω ∈ s → all_stream' (stream.tail ω) → all_stream' ω
 
 
 coinductive alt_stream : stream bool → Prop
@@ -55,3 +55,29 @@ with ff_stream : stream bool → Prop
     (∀ (a : stream bool), C_tt_stream a → tt_stream.functional C_tt_stream C_ff_stream a) →
     (∀ (a : stream bool), C_ff_stream a → ff_stream.functional C_tt_stream C_ff_stream a) →
     ∀ (a : stream bool), C_ff_stream a → ff_stream a)
+
+
+mutual coinductive tt_ff_stream, ff_tt_stream
+with tt_ff_stream : stream bool → Prop
+| step {} : ∀{ω : stream bool}, tt_ff_stream ω ∨ ff_tt_stream ω → tt_ff_stream (stream.cons tt ω)
+with ff_tt_stream : stream bool → Prop
+| step {} : ∀{ω : stream bool}, ff_tt_stream ω ∨ tt_ff_stream ω → ff_tt_stream (stream.cons ff ω)
+
+#print prefix tt_ff_stream
+
+inductive all_list {α : Type} (p : α → Prop) : list α → Prop
+| nil  : all_list []
+| cons : ∀a xs, p a → all_list xs → all_list (a :: xs)
+
+@[monotonicity]
+lemma monotonicity.all_list {α : Type} {p q : α → Prop} (h : ∀a, implies (p a) (q a)) :
+  ∀xs, implies (all_list p xs) (all_list q xs)
+| ._ (all_list.nil ._)           := all_list.nil _
+| ._ (all_list.cons a xs ha hxs) := all_list.cons _ _ (h a ha) (monotonicity.all_list _ hxs)
+
+mutual coinductive walk_a, walk_b {α β : Type} (f : α → list β) (g : β → α) (p : α → Prop) (t : α → Prop)
+with walk_a : α → Prop
+| step : ∀a, all_list walk_b (f a) → p a → walk_a a
+| term : ∀a, t a → walk_a a
+with walk_b : β → Prop
+| step : ∀b, walk_a (g b) → walk_b b
